barrier/client.v
@@ -5,10 +5,8 @@ Import uPred.
 Definition client := (let: "b" := newchan '() in wait "b")%L.
 
 Section client.
-  Context {Σ : iFunctorG} (N : namespace).
-  Context `{heapG Σ} (heapN : namespace).
-  (* TODO: This should be abstracted away somehow. *)
-  Context `{inGF heap_lang Σ (stsGF barrier_proto.sts)} `{inGF heap_lang Σ agreeF}.
+  Context {Σ : iFunctorG} `{!heapG Σ} `{!barrierG Σ}.
+  Context (N : namespace) (heapN : namespace).
 
   Local Notation iProp := (iPropG heap_lang Σ).
 
